1. bidirectional G and refine_env 2. updated wf conditions

src/Framework/Checking.v
@@ -6,9 +6,7 @@ Import ListNotations.
 Require Import Lia.
 From Hammer Require Import Hammer Tactics Reflect.
 
-From Framework Require Import Util W0 ANF1 ANF.
-
-Module AS := ANF1.
+From Framework Require Import Util W0 ANF ANF1.
 
 Definition web_map := M.t web.
 
@@ -22,7 +20,7 @@ Hint Constructors tag : core.
 
 (* Value *)
 Inductive cval : Type :=
-| CVfun : var -> M.t (ctag cval) -> list var -> AS.exp -> cval
+| CVfun : var -> M.t (ctag cval) -> list var -> exp -> cval
 | CVconstr : ctor_tag -> list (ctag cval) -> cval.
 
 Hint Constructors cval : core.
@@ -122,17 +120,17 @@ Hint Constructors wf_cres : core.
 
 (* Checking Semantics *)
 (* `W` is a valid analysis result with respect to the checking big-step semantics *)
-Inductive cbstep (W : web_map) (ex : bool) (ρ : cenv) : AS.exp -> fuel -> cres -> Prop :=
+Inductive cbstep (W : web_map) (ex : bool) (ρ : cenv) : exp -> fuel -> cres -> Prop :=
 | Cbstep_ret :
   forall {x v},
     M.get x ρ = Some v ->
-    cbstep W ex ρ (AS.Eret x) 0 (CRes v)
+    cbstep W ex ρ (Eret x) 0 (CRes v)
 
 | Cbstep_fun :
   forall {f l w xs e k c r},
     W ! l = Some w ->
     cbstep_fuel W ex (M.set f (CTag l W (CVfun f ρ xs e)) ρ) k c r ->
-    cbstep W ex ρ (AS.Efun f l xs e k) c r
+    cbstep W ex ρ (Efun f l xs e k) c r
 
 | Cbstep_app :
   forall {W' f f' l l' w xs ρ' xs' e vs ρ'' c r},
@@ -143,7 +141,7 @@ Inductive cbstep (W : web_map) (ex : bool) (ρ : cenv) : AS.exp -> fuel -> cres 
     W' ! l' = Some w -> (* W' controls callee *)
     (w \in Exposed -> Forall to_exposed vs /\ to_exposed_cres r) -> (* Doesn't matter which W as long as `vs` and `r` are mapped to exposed web ids. *)
     cbstep_fuel W' (exposedb w) ρ'' e c r ->
-    cbstep W ex ρ (AS.Eapp f l xs) c r
+    cbstep W ex ρ (Eapp f l xs) c r
 
 | Cbstep_letapp_Res :
   forall {W' x f f' l l' w xs k ρ' xs' e vs ρ'' c c' v r},
@@ -155,7 +153,7 @@ Inductive cbstep (W : web_map) (ex : bool) (ρ : cenv) : AS.exp -> fuel -> cres 
     cbstep_fuel W' (exposedb w) ρ'' e c (CRes v) ->
     cbstep_fuel W ex (M.set x v ρ) k c' r ->
     (w \in Exposed -> Forall to_exposed vs /\ to_exposed v) ->
-    cbstep W ex ρ (AS.Eletapp x f l xs k) (c + c') r
+    cbstep W ex ρ (Eletapp x f l xs k) (c + c') r
 
 | Cbstep_letapp_OOT :
   forall {W' x f f' l l' w xs k ρ' xs' e vs ρ'' c},
@@ -166,7 +164,7 @@ Inductive cbstep (W : web_map) (ex : bool) (ρ : cenv) : AS.exp -> fuel -> cres 
     W' ! l' = Some w ->
     cbstep_fuel W' (exposedb w) ρ'' e c COOT ->
     (w \in Exposed -> Forall to_exposed vs) ->
-    cbstep W ex ρ (AS.Eletapp x f l xs k) c COOT
+    cbstep W ex ρ (Eletapp x f l xs k) c COOT
 
 | Cbstep_constr :
   forall {x l w t xs e r vs c},
@@ -174,7 +172,7 @@ Inductive cbstep (W : web_map) (ex : bool) (ρ : cenv) : AS.exp -> fuel -> cres 
     W ! l = Some w ->
     (w \in Exposed -> Forall to_exposed vs) ->
     cbstep_fuel W ex (M.set x (CTag l W (CVconstr t vs)) ρ) e c r ->
-    cbstep W ex ρ (AS.Econstr x l t xs e) c r
+    cbstep W ex ρ (Econstr x l t xs e) c r
 
 | Cbstep_proj :
   forall {W' x l l' w t i y e c r v vs},
@@ -183,7 +181,7 @@ Inductive cbstep (W : web_map) (ex : bool) (ρ : cenv) : AS.exp -> fuel -> cres 
     W ! l = Some w ->
     W' ! l' = Some w ->
     cbstep_fuel W ex (M.set x v ρ) e c r ->
-    cbstep W ex ρ (AS.Eproj x l i y e) c r
+    cbstep W ex ρ (Eproj x l i y e) c r
 
 | Cbstep_case :
   forall {W' x l l' w cl t e r c vs},
@@ -192,9 +190,9 @@ Inductive cbstep (W : web_map) (ex : bool) (ρ : cenv) : AS.exp -> fuel -> cres 
     W ! l = Some w ->
     W' ! l' = Some w ->
     cbstep_fuel W ex ρ e c r ->
-    cbstep W ex ρ (AS.Ecase x l cl) c r
+    cbstep W ex ρ (Ecase x l cl) c r
 
-with cbstep_fuel (W : web_map) (ex : bool) (ρ : cenv) : AS.exp -> fuel -> cres -> Prop :=
+with cbstep_fuel (W : web_map) (ex : bool) (ρ : cenv) : exp -> fuel -> cres -> Prop :=
 | CbstepF_OOT :
   forall {e},
     cbstep_fuel W ex ρ e 0 COOT
@@ -550,7 +548,7 @@ Inductive csubval : clval -> clval -> Prop :=
 with csubval' : cval -> cval -> Prop :=
 | CSub_fun :
   forall Γ f xs e ρ1 ρ2,
-    (AS.occurs_free e) \subset (FromList xs :|: (f |: Γ)) ->
+    (occurs_free e) \subset (FromList xs :|: (f |: Γ)) ->
     csubenv Γ ρ1 ρ2 ->
     csubval' (CVfun f ρ1 xs e) (CVfun f ρ2 xs e)
 
@@ -772,14 +770,14 @@ Proof.
   induction H using wf_cval_mut with
     (P0 := fun v wf =>
              match v with
-             | CVfun f ρ xs e => csubenv (AS.occurs_free e) ρ ρ
+             | CVfun f ρ xs e => csubenv (occurs_free e) ρ ρ
              | CVconstr c vs => Forall2 csubval vs vs
              end)
     (P1 := fun ρ wf => forall Γ, csubenv Γ ρ ρ);
     eauto.
   - destruct v.
     + constructor; auto.
-      eapply (CSub_fun (AS.occurs_free e0)); eauto.
+      eapply (CSub_fun (occurs_free e0)); eauto.
       unfold Ensembles.Included, Ensembles.In, FromList.
       intros.
       repeat apply Union_intror; auto.
@@ -806,7 +804,7 @@ Qed.
 (* Semantic Weakening for the Checking Semantics *)
 Lemma cbstep_subenv {W ex Γ ρ1 ρ2 e c r1}:
   wf_cenv ρ2 ->
-  (AS.occurs_free e) \subset Γ ->
+  (occurs_free e) \subset Γ ->
   csubenv Γ ρ1 ρ2 ->
   cbstep W ex ρ1 e c r1 ->
   (exists r2, cbstep W ex ρ2 e c r2 /\ csubres r1 r2 /\ wf_cres r2).
@@ -817,7 +815,7 @@ Proof.
   induction H1 using cbstep_ind' with
     (P0 := fun W ex ρ1 e c r1 =>
              forall Γ,
-               AS.occurs_free e \subset Γ ->
+               occurs_free e \subset Γ ->
                forall ρ2,
                  wf_cenv ρ2 ->
                  csubenv Γ ρ1 ρ2 ->
@@ -831,8 +829,8 @@ Proof.
     eapply wf_cenv_get; eauto.
 
   - (* Cbstep_fun *)
-    assert (HFk : AS.occurs_free k \subset (f |: Γ)) by (eapply AS.free_fun_k_inv; eauto).
-    assert (HFe : AS.occurs_free e \subset FromList xs :|: (f |: Γ)) by (eapply AS.free_fun_e_inv; eauto).
+    assert (HFk : occurs_free k \subset (f |: Γ)) by (eapply free_fun_k_inv; eauto).
+    assert (HFe : occurs_free e \subset FromList xs :|: (f |: Γ)) by (eapply free_fun_e_inv; eauto).
     rename W into W0.
     set (clos1 := CTag l W0 (CVfun f ρ xs e)).
     set (clos2 := CTag l W0 (CVfun f ρ2 xs e)).
@@ -856,7 +854,7 @@ Proof.
     inv H12.
     edestruct (csubenv_get_lists H7 xs) as [vs2 [Heqvs2 Hvs2]]; eauto.
     eapply Included_trans; eauto.
-    apply AS.free_app_xs_subset.
+    apply free_app_xs_subset.
 
     assert (Hlen : length xs' = length vs2).
     { erewrite <- (Forall2_length _ _ _ Hvs2); eauto.
@@ -894,7 +892,7 @@ Proof.
     inv H13.
     edestruct (csubenv_get_lists H8 xs) as [vs2 [Heqvs2 Hvs2]]; eauto.
     eapply Included_trans; eauto.
-    apply AS.free_letapp_xs_subset.
+    apply free_letapp_xs_subset.
 
     assert (Hlen : length xs' = length vs2).
     { erewrite <- (Forall2_length _ _ _ Hvs2); eauto.
@@ -919,7 +917,7 @@ Proof.
       eapply csubenv_set; eauto. }
     edestruct (IHcbstep _ H15 ρ2'') as [r2 [Hr2 [Hs Hr]]]; eauto.
     inv Hs.
-    assert (HFk : AS.occurs_free k \subset (x |: Γ)) by (eapply AS.free_letapp_k_inv; eauto).
+    assert (HFk : occurs_free k \subset (x |: Γ)) by (eapply free_letapp_k_inv; eauto).
     edestruct (IHcbstep0 _ HFk (M.set x v2 ρ2)) as [r3 [Hr3 [Hs' Hr']]].
     + eapply wf_cenv_set; eauto. inv Hr; auto.
     + eapply csubenv_set; eauto.
@@ -938,7 +936,7 @@ Proof.
     inv H12.
     edestruct (csubenv_get_lists H7 xs) as [vs2 [Heqvs2 Hvs2]]; eauto.
     eapply Included_trans; eauto.
-    apply AS.free_letapp_xs_subset.
+    apply free_letapp_xs_subset.
 
     assert (Hlen : length xs' = length vs2).
     { erewrite <- (Forall2_length _ _ _ Hvs2); eauto.
@@ -970,9 +968,9 @@ Proof.
   - (* Cbstep_constr *)
     edestruct (csubenv_get_lists H4 xs) as [vs2 [Heqvs2 Hvs2]]; eauto.
     eapply Included_trans; eauto.
-    apply AS.free_constr_xs_subset.
+    apply free_constr_xs_subset.
 
-    assert (HFk : AS.occurs_free e \subset (x |: Γ)) by (eapply AS.free_constr_k_inv; eauto).
+    assert (HFk : occurs_free e \subset (x |: Γ)) by (eapply free_constr_k_inv; eauto).
     rename W into W0.
     edestruct (IHcbstep _ HFk (M.set x (CTag l W0 (CVconstr t vs2)) ρ2))
       as [r2 [Hr2 [Hs Hr]]].
@@ -990,7 +988,7 @@ Proof.
     edestruct (csubenv_get H5 y) as [vy2 [Heqvy2 Hvy2]]; eauto.
     edestruct (csubval_CVconstr_inv_l Hvy2) as [vs2 [Heqvs2 Hvs2]]; subst.
     edestruct (Forall2_nth_error H0 Hvs2) as [v' [Heqv' Hv]].
-    assert (HFk : AS.occurs_free e \subset (x |: Γ)) by (eapply AS.free_proj_k_inv; eauto).
+    assert (HFk : occurs_free e \subset (x |: Γ)) by (eapply free_proj_k_inv; eauto).
     edestruct (IHcbstep _ HFk (M.set x v' ρ2)) as [r2 [Hr2 [Hs Hr]]].
     + eapply wf_cenv_set; eauto.
       assert (Hwfvy : wf_cval (CTag l' W' (CVconstr t vs2))) by (eapply wf_cenv_get; eauto).
@@ -1005,7 +1003,7 @@ Proof.
     edestruct (csubenv_get H5 x) as [vx2 [Heqvx2 Hvx2]]; eauto.
     edestruct (csubval_CVconstr_inv_l Hvx2) as [vs2 [Heqvs2 Hvs2]]; subst.
     edestruct IHcbstep as [r2 [Hr2 [Hs Hr]]]; eauto.
-    + eapply AS.free_case_e_inv; eauto.
+    + eapply free_case_e_inv; eauto.
 
   - (* CbstepF_OOT *)
     exists COOT; repeat split; auto.
@@ -1019,7 +1017,7 @@ Qed.
 
 Lemma cbstep_fuel_subenv {W ex Γ ρ1 ρ2 e c r1}:
   wf_cenv ρ2 ->
-  (AS.occurs_free e) \subset Γ ->
+  (occurs_free e) \subset Γ ->
   csubenv Γ ρ1 ρ2 ->
   cbstep_fuel W ex ρ1 e c r1 ->
   (exists r2, cbstep_fuel W ex ρ2 e c r2 /\ csubres r1 r2 /\ wf_cres r2).
@@ -1034,30 +1032,30 @@ Proof.
 Qed.
 
 (* Value Refinement *)
-Inductive refine_val : AS.wval -> clval -> Prop :=
+Inductive refine_val : wval -> clval -> Prop :=
 | Refine_wval :
   forall l v v' W,
     refine_val' v v' ->
-    refine_val (AS.Tag l v) (CTag l W v')
+    refine_val (Tag l v) (CTag l W v')
 
-with refine_val' : AS.val -> cval -> Prop :=
+with refine_val' : val -> cval -> Prop :=
 | Refine_fun :
   forall Γ f ρ ρ' xs e,
-    (AS.occurs_free e) \subset (FromList xs :|: (f |: Γ)) ->
+    (occurs_free e) \subset (FromList xs :|: (f |: Γ)) ->
     refine_env Γ ρ ρ' ->
-    refine_val' (AS.Vfun f ρ xs e) (CVfun f ρ' xs e)
+    refine_val' (Vfun f ρ xs e) (CVfun f ρ' xs e)
 
 | Refine_constr_nil :
   forall c,
-    refine_val' (AS.Vconstr c []) (CVconstr c [])
+    refine_val' (Vconstr c []) (CVconstr c [])
 
 | Refine_constr :
   forall c v vs v' vs',
     refine_val v v' ->
-    refine_val' (AS.Vconstr c vs) (CVconstr c vs') ->
-    refine_val' (AS.Vconstr c (v :: vs)) (CVconstr c (v' :: vs'))
+    refine_val' (Vconstr c vs) (CVconstr c vs') ->
+    refine_val' (Vconstr c (v :: vs)) (CVconstr c (v' :: vs'))
 
-with refine_env : vars -> AS.env -> cenv -> Prop :=
+with refine_env : vars -> env -> cenv -> Prop :=
 | Refine_env :
   forall Γ ρ ρ',
     (forall x,
@@ -1076,14 +1074,14 @@ Scheme refine_val_mut := Induction for refine_val Sort Prop
 with refine_val'_mut := Induction for refine_val' Sort Prop
 with refine_env_mut := Induction for refine_env Sort Prop.
 
-Inductive refine_res : AS.res -> cres -> Prop :=
+Inductive refine_res : res -> cres -> Prop :=
 | Refine_COOT :
-  refine_res AS.OOT COOT
+  refine_res OOT COOT
 
 | Refine_CRes :
   forall v v',
     refine_val v v' ->
-    refine_res (AS.Res v) (CRes v').
+    refine_res (Res v) (CRes v').
 
 Hint Constructors refine_res : core.
 
@@ -1175,10 +1173,10 @@ Proof.
 Qed.
 
 Lemma refine_val_Vfun_inv {l f ρ xs e v''} :
-  refine_val (AS.Tag l (AS.Vfun f ρ xs e)) v'' ->
+  refine_val (Tag l (Vfun f ρ xs e)) v'' ->
   exists W ρ' Γ,
     v'' = CTag l W (CVfun f ρ' xs e) /\
-    AS.occurs_free e \subset (FromList xs :|: (f |: Γ)) /\
+    occurs_free e \subset (FromList xs :|: (f |: Γ)) /\
     refine_env Γ ρ ρ'.
 Proof.
   intros H.
@@ -1188,10 +1186,10 @@ Proof.
 Qed.
 
 Lemma refine_val'_Vconstr_inv {t vs v''} :
-  refine_val' (AS.Vconstr t vs) v'' ->
+  refine_val' (Vconstr t vs) v'' ->
   exists vs', v'' = CVconstr t vs' /\ Forall2 refine_val vs vs'.
 Proof.
-  intros H. remember (AS.Vconstr t vs) as v0 eqn:Heq.
+  intros H. remember (Vconstr t vs) as v0 eqn:Heq.
   revert t vs Heq.
   induction H; intros t0 vs0 Heq; inv Heq.
   - exists []; split; auto.
@@ -1200,7 +1198,7 @@ Proof.
 Qed.
 
 Lemma refine_val_Vconstr_inv {l t vs v''} :
-  refine_val (AS.Tag l (AS.Vconstr t vs)) v'' ->
+  refine_val (Tag l (Vconstr t vs)) v'' ->
   exists W vs', v'' = CTag l W (CVconstr t vs') /\ Forall2 refine_val vs vs'.
 Proof.
   intros H. inv H. apply refine_val'_Vconstr_inv in H3 as [vs' [-> Hr]]; eauto.
@@ -1208,12 +1206,12 @@ Qed.
 
 Lemma refine_val'_Vconstr {t vs vs'} :
   Forall2 refine_val vs vs' ->
-  refine_val' (AS.Vconstr t vs) (CVconstr t vs').
+  refine_val' (Vconstr t vs) (CVconstr t vs').
 Proof. intros Hr. induction Hr; auto. Qed.
 
 Lemma refine_val_Vconstr {l W t vs vs'} :
   Forall2 refine_val vs vs' ->
-  refine_val (AS.Tag l (AS.Vconstr t vs)) (CTag l W (CVconstr t vs')).
+  refine_val (Tag l (Vconstr t vs)) (CTag l W (CVconstr t vs')).
 Proof. intros Hr. constructor. apply refine_val'_Vconstr; auto. Qed.
 
 (* [refine_val] commutes with [subval] *)
@@ -1285,15 +1283,15 @@ Qed.
 
 Lemma refine_val_subval v0 v0' v :
   refine_val v0 v ->
-  AS.subval v0 v0' ->
+  subval v0 v0' ->
   refine_val v0' v
 with refine_val'_subval' v0 v0' v :
   refine_val' v0 v ->
-  AS.subval' v0 v0' ->
+  subval' v0 v0' ->
   refine_val' v0' v
 with refine_env_subenv Γ Γ' ρa ρa' ρc :
   refine_env Γ ρa ρc ->
-  AS.subenv Γ' ρa ρa' ->
+  subenv Γ' ρa ρa' ->
   refine_env (Γ :&: Γ') ρa' ρc.
 Proof.
   - (* refine_val_subval *)
@@ -1340,7 +1338,7 @@ Qed.
 
 Lemma refine_res_subres r0 r0' r :
   refine_res r0 r ->
-  AS.subres r0 r0' ->
+  subres r0 r0' ->
   refine_res r0' r.
 Proof.
   intros Hr Hs.
@@ -1351,27 +1349,27 @@ Qed.
 
 (* Correlation lemmas: bstep and cbstep that both terminate on the same expression agree on fuel and value. *)
 Lemma bstep_cbstep_aux v1 v2 {W ex ρ1 ρ2 e c1 r1 c2 r2} :
-  AS.bstep ρ1 e c1 r1 ->
-  refine_env (AS.occurs_free e) ρ1 ρ2 ->
+  bstep ρ1 e c1 r1 ->
+  refine_env (occurs_free e) ρ1 ρ2 ->
   cbstep W ex ρ2 e c2 r2 ->
-  r1 = AS.Res v1 ->
+  r1 = Res v1 ->
   r2 = CRes v2 ->
   c1 = c2 /\ refine_val v1 v2.
 Proof.
   intros Hb.
   revert v1 v2 ρ2 W ex c2 r2.
-  induction Hb using AS.bstep_ind'
+  induction Hb using bstep_ind'
     with (P := fun ρ1 e c1 r1 =>
                  forall v1 v2 ρ2 W ex c2 r2,
-                   refine_env (AS.occurs_free e) ρ1 ρ2 ->
+                   refine_env (occurs_free e) ρ1 ρ2 ->
                    cbstep W ex ρ2 e c2 r2 ->
-                   r1 = AS.Res v1 -> r2 = CRes v2 ->
+                   r1 = Res v1 -> r2 = CRes v2 ->
                    c1 = c2 /\ refine_val v1 v2)
          (P0 := fun ρ1 e c1 r1 =>
                   forall v1 v2 ρ2 W ex c2 r2,
-                    refine_env (AS.occurs_free e) ρ1 ρ2 ->
+                    refine_env (occurs_free e) ρ1 ρ2 ->
                     cbstep_fuel W ex ρ2 e c2 r2 ->
-                    r1 = AS.Res v1 -> r2 = CRes v2 ->
+                    r1 = Res v1 -> r2 = CRes v2 ->
                     c1 = c2 /\ refine_val v1 v2);
     intros v1 v2 ρ2 W0 ex c2 r2 Henv Hc Heq1 Heq2; subst.
 
@@ -1382,21 +1380,21 @@ Proof.
 
   - (* BStep_fun: FV(Efun f l xs e_body k) *)
     inv Hc.
-    assert (Href_clos : refine_val (AS.Tag w (AS.Vfun f ρ xs e))
+    assert (Href_clos : refine_val (Tag w (Vfun f ρ xs e))
                           (CTag w W0 (CVfun f ρ2 xs e))).
     { constructor. econstructor.
-      - eapply AS.free_fun_e_inv. apply Included_refl.
+      - eapply free_fun_e_inv. apply Included_refl.
       - exact Henv. }
     eapply IHHb.
     + (* FV(k) ⊆ f |: FV(Efun) via free_fun_k_subset; refine_env_set + subset *)
       eapply refine_env_subset.
       * eapply refine_env_set; eauto.
-      * apply AS.free_fun_k_subset.
+      * apply free_fun_k_subset.
     + eauto. + eauto. + eauto.
 
   - (* BStep_app: FV(Eapp f l xs) = {f} ∪ xs *)
     inv Hc.
-    edestruct (refine_env_get f (AS.Tag w' (AS.Vfun f' ρ' xs' e)) Henv (ltac:(constructor)) H) as [vf [Hvf Hrf]].
+    edestruct (refine_env_get f (Tag w' (Vfun f' ρ' xs' e)) Henv (ltac:(constructor)) H) as [vf [Hvf Hrf]].
     invc.
     destruct (refine_val_Vfun_inv Hrf) as [W'' [ρ_2' [Γ_c [Heq [HFVe Hre]]]]].
     inv Heq.
@@ -1404,11 +1402,11 @@ Proof.
                  (ltac:(unfold Ensembles.Included, Ensembles.In; intros z Hz; constructor; auto))
                  H0) as [vs2 [Hvs2 Hrvs]].
     invc.
-    assert (Href_f : refine_val (AS.Tag w' (AS.Vfun f' ρ' xs' e))
+    assert (Href_f : refine_val (Tag w' (Vfun f' ρ' xs' e))
                        (CTag w' W'' (CVfun f' ρ_2' xs' e))).
     { constructor. econstructor; eauto. }
     assert (Hrenv : refine_env (f' |: Γ_c)
-                      (M.set f' (AS.Tag w' (AS.Vfun f' ρ' xs' e)) ρ')
+                      (M.set f' (Tag w' (Vfun f' ρ' xs' e)) ρ')
                       (M.set f' (CTag w' W'' (CVfun f' ρ_2' xs' e)) ρ_2')).
     { apply refine_env_set; eauto. }
     pose proof (refine_env_set_lists xs' vs vs2 Hrvs Hrenv H1 H8) as Hre''.
@@ -1418,19 +1416,19 @@ Proof.
   - (* BStep_letapp_Res *)
     inv Hc.
     + (* Cbstep_letapp_Res *)
-      edestruct (refine_env_get f (AS.Tag w' (AS.Vfun f' ρ' xs' e)) Henv (ltac:(apply AS.Free_letapp2)) H) as [vf [Hvf Hrf]].
+      edestruct (refine_env_get f (Tag w' (Vfun f' ρ' xs' e)) Henv (ltac:(apply Free_letapp2)) H) as [vf [Hvf Hrf]].
       invc.
       destruct (refine_val_Vfun_inv Hrf) as [W'' [ρ_2' [Γ_c [Heq [HFVe Hre]]]]].
       inv Heq.
-      assert (Hxs_in : FromList xs \subset AS.occurs_free (AS.Eletapp x f w xs k))
-        by (apply AS.free_letapp_xs_subset).
+      assert (Hxs_in : FromList xs \subset occurs_free (Eletapp x f w xs k))
+        by (apply free_letapp_xs_subset).
       edestruct (refine_env_get_list xs _ Henv Hxs_in H0) as [vs2 [Hvs2 Hrvs]].
       invc.
-      assert (Href_f : refine_val (AS.Tag w' (AS.Vfun f' ρ' xs' e))
+      assert (Href_f : refine_val (Tag w' (Vfun f' ρ' xs' e))
                            (CTag w' W'' (CVfun f' ρ_2' xs' e))).
         { constructor. econstructor; eauto. }
         assert (Hrenv : refine_env (f' |: Γ_c)
-                          (M.set f' (AS.Tag w' (AS.Vfun f' ρ' xs' e)) ρ')
+                          (M.set f' (Tag w' (Vfun f' ρ' xs' e)) ρ')
                           (M.set f' (CTag w' W'' (CVfun f' ρ_2' xs' e)) ρ_2')).
         { apply refine_env_set; eauto. }
         pose proof (refine_env_set_lists xs' vs vs2 Hrvs Hrenv H1 H11) as Hre''.
@@ -1439,7 +1437,7 @@ Proof.
         edestruct (IHHb0 v1 v2) as [Hc0' Hrv2]; eauto.
         { eapply refine_env_subset.
           - apply refine_env_set; eauto.
-          - apply AS.free_letapp_k_subset. }
+          - apply free_letapp_k_subset. }
 
   - fcrush.
 
@@ -1452,11 +1450,11 @@ Proof.
     eapply IHHb; eauto.
     eapply refine_env_subset.
     + apply refine_env_set; [exact Henv | apply refine_val_Vconstr; auto].
-    + apply AS.free_constr_k_subset.
+    + apply free_constr_k_subset.
 
   - (* BStep_proj: FV(Eproj x l i y e) *)
     inv Hc.
-    edestruct (refine_env_get y (AS.Tag w' (AS.Vconstr t vs)) Henv (ltac:(constructor)) H) as [vc [Hvc Hrc]].
+    edestruct (refine_env_get y (Tag w' (Vconstr t vs)) Henv (ltac:(constructor)) H) as [vc [Hvc Hrc]].
     invc.
       destruct (refine_val_Vconstr_inv Hrc) as [W'' [vs' [Heq Hrvs]]].
       inv Heq.
@@ -1465,18 +1463,18 @@ Proof.
       eapply IHHb; eauto.
       eapply refine_env_subset.
       * apply refine_env_set; [exact Henv | exact Hrv'].
-      * apply AS.free_proj_k_subset.
+      * apply free_proj_k_subset.
 
   - (* BStep_case *)
     inv Hc.
-    edestruct (refine_env_get x (AS.Tag w' (AS.Vconstr t vs)) Henv (ltac:(constructor)) H) as [vc [Hvc Hrc]].
+    edestruct (refine_env_get x (Tag w' (Vconstr t vs)) Henv (ltac:(constructor)) H) as [vc [Hvc Hrc]].
     invc.
       destruct (refine_val_Vconstr_inv Hrc) as [W'' [vs' [Heq _]]].
       inv Heq.
       destruct (find_tag_deterministic H0 H6); subst.
       eapply IHHb; eauto.
       eapply refine_env_subset; [exact Henv |].
-      eapply AS.free_case_e_inv; eauto. apply Included_refl.
+      eapply free_case_e_inv; eauto. apply Included_refl.
 
   - discriminate.
 
@@ -1484,15 +1482,15 @@ Proof.
 Qed.
 
 Lemma bstep_cbstep_refine W ex ρ1 ρ2 e c1 c2 v1 v2 :
-  AS.bstep ρ1 e c1 (AS.Res v1) ->
-  refine_env (AS.occurs_free e) ρ1 ρ2 ->
+  bstep ρ1 e c1 (Res v1) ->
+  refine_env (occurs_free e) ρ1 ρ2 ->
   cbstep W ex ρ2 e c2 (CRes v2) ->
   c1 = c2 /\ refine_val v1 v2.
 Proof. intros; eapply bstep_cbstep_aux; eauto. Qed.
 
 Lemma bstep_fuel_cbstep_fuel_refine W ex ρ1 ρ2 e c1 c2 v1 v2 :
-  AS.bstep_fuel ρ1 e c1 (AS.Res v1) ->
-  refine_env (AS.occurs_free e) ρ1 ρ2 ->
+  bstep_fuel ρ1 e c1 (Res v1) ->
+  refine_env (occurs_free e) ρ1 ρ2 ->
   cbstep_fuel W ex ρ2 e c2 (CRes v2) ->
   c1 = c2 /\ refine_val v1 v2.
 Proof.
@@ -1502,25 +1500,25 @@ Qed.
 
 (* Valid web_map Specification *)
 (* This essentially says `has_label e` ⊆ Dom_map W *)
-Inductive web_map_spec (W : web_map) (Γ : vars) : AS.exp -> Prop :=
+Inductive web_map_spec (W : web_map) (Γ : vars) : exp -> Prop :=
 | Web_Map_Spec_ret :
   forall x,
     (x \in Γ) ->
-    web_map_spec W Γ (AS.Eret x)
+    web_map_spec W Γ (Eret x)
 
 | Web_Map_Spec_fun :
   forall {f l w xs e k},
     W ! l = Some w ->
     web_map_spec W (FromList xs :|: (f |: Γ)) e ->
     web_map_spec W (f |: Γ) k ->
-    web_map_spec W Γ (AS.Efun f l xs e k)
+    web_map_spec W Γ (Efun f l xs e k)
 
 | Web_Map_Spec_app :
   forall {f l w xs},
     W ! l = Some w ->
     (f \in Γ) ->
     (FromList xs \subset Γ) ->
-    web_map_spec W Γ (AS.Eapp f l xs)
+    web_map_spec W Γ (Eapp f l xs)
 
 | Web_Map_Spec_letapp :
   forall {x f l w xs k},
@@ -1528,82 +1526,82 @@ Inductive web_map_spec (W : web_map) (Γ : vars) : AS.exp -> Prop :=
     (f \in Γ) ->
     (FromList xs \subset Γ) ->
     web_map_spec W (x |: Γ) k ->
-    web_map_spec W Γ (AS.Eletapp x f l xs k)
+    web_map_spec W Γ (Eletapp x f l xs k)
 
 | Web_Map_Spec_constr :
   forall {x l w t xs k},
     W ! l = Some w ->
     (FromList xs \subset Γ) ->
     web_map_spec W (x |: Γ) k ->
-    web_map_spec W Γ (AS.Econstr x l t xs k)
+    web_map_spec W Γ (Econstr x l t xs k)
 
 | Web_Map_Spec_proj :
   forall {l w x y k n},
     W ! l = Some w ->
     (y \in Γ) ->
     web_map_spec W (x |: Γ) k ->
-    web_map_spec W Γ (AS.Eproj x l n y k)
+    web_map_spec W Γ (Eproj x l n y k)
 
 | Web_Map_Spec_case_nil :
   forall {l w x},
     W ! l = Some w ->
     (x \in Γ) ->
-    web_map_spec W Γ (AS.Ecase x l [])
+    web_map_spec W Γ (Ecase x l [])
 
 | Web_Map_Spec_case_cons :
   forall {x l w e t cl},
     W ! l = Some w ->
     (x \in Γ) ->
     web_map_spec W Γ e ->
-    web_map_spec W Γ (AS.Ecase x l cl) ->
-    web_map_spec W Γ (AS.Ecase x l ((t, e) :: cl)).
+    web_map_spec W Γ (Ecase x l cl) ->
+    web_map_spec W Γ (Ecase x l ((t, e) :: cl)).
 
 Hint Constructors web_map_spec : core.
 
 Lemma web_map_total W e :
   (has_label e \subset Dom_map W) ->
-  web_map_spec W (AS.occurs_free e) e.
+  web_map_spec W (occurs_free e) e.
 Proof.
   enough (Hstrong : forall Γ,
              has_label e \subset Dom_map W ->
-             AS.occurs_free e \subset Γ ->
+             occurs_free e \subset Γ ->
              web_map_spec W Γ e).
   { intros; apply Hstrong; auto; apply Included_refl. }
-  induction e using AS.exp_ind'; intros Γ Hlabel Hfree.
+  induction e using exp_ind'; intros Γ Hlabel Hfree.
   - (* Eret x *)
     constructor. apply Hfree. constructor.
   - (* Eapp x w xs *)
     assert (Hl : w \in Dom_map W) by (apply Hlabel; auto).
     destruct Hl as [web Hw].
     econstructor; eauto.
-    eapply AS.free_app_xs_inv; eauto.
+    eapply free_app_xs_inv; eauto.
   - (* Efun f w xs e k *)
     assert (Hl : w \in Dom_map W) by (apply Hlabel; auto).
     destruct Hl as [web Hw].
     econstructor; eauto.
     + apply IHe1.
       * eauto using Included_trans, has_label_fun_body.
-      * eapply AS.free_fun_e_inv; eauto.
+      * eapply free_fun_e_inv; eauto.
     + apply IHe2.
       * eauto using Included_trans, has_label_fun_cont.
-      * eapply AS.free_fun_k_inv; eauto.
+      * eapply free_fun_k_inv; eauto.
   - (* Eletapp x f w xs k *)
     assert (Hl : w \in Dom_map W) by (apply Hlabel; auto).
     destruct Hl as [web Hw].
     econstructor; eauto.
-    + eapply AS.free_letapp_xs_inv; eauto.
+    + eapply free_letapp_xs_inv; eauto.
     + apply IHe.
       * eauto using Included_trans, has_label_letapp_cont.
-      * eapply AS.free_letapp_k_inv; eauto.
+      * eapply free_letapp_k_inv; eauto.
   - (* Econstr x w c xs k *)
     assert (Hl : w \in Dom_map W) by (apply Hlabel; auto).
     destruct Hl as [web Hw].
     econstructor; eauto.
     + eapply Included_trans; eauto.
-      eapply AS.free_constr_xs_subset; eauto.
+      eapply free_constr_xs_subset; eauto.
     + apply IHe.
       * eauto using Included_trans, has_label_constr_cont.
-      * eapply AS.free_constr_k_inv; eauto.
+      * eapply free_constr_k_inv; eauto.
   - (* Ecase x w [] *)
     assert (Hl : w \in Dom_map W) by (apply Hlabel; auto).
     destruct Hl as [web Hw].
@@ -1615,32 +1613,32 @@ Proof.
     + apply IHe.
       * eauto using Included_trans, has_label_case_hd.
       * eapply Included_trans; eauto.
-        eapply AS.free_case_hd_subset.
+        eapply free_case_hd_subset.
     + apply IHe0.
       * eauto using Included_trans, has_label_case_tl.
       * eapply Included_trans; eauto.
-        apply AS.free_case_tl_subset.
+        apply free_case_tl_subset.
   - (* Eproj x w n v0 e *)
     assert (Hl : w \in Dom_map W) by (apply Hlabel; auto).
     destruct Hl as [web Hw].
     econstructor; eauto.
     + apply IHe.
       * eauto using Included_trans, has_label_proj_body.
-      * eapply AS.free_proj_k_inv; eauto.
+      * eapply free_proj_k_inv; eauto.
 Qed.
 
 (* Cross-semantics Logical Relations *)
-Definition R' (P : nat -> AS.wval -> clval -> Prop) (i : nat) (r1 : AS.res) (r2 : cres) :=
+Definition R' (P : nat -> wval -> clval -> Prop) (i : nat) (r1 : res) (r2 : cres) :=
   match r1, r2 with
-  | AS.OOT, COOT => True
-  | AS.Res v1, CRes v2 => P i v1 v2
+  | OOT, COOT => True
+  | Res v1, CRes v2 => P i v1 v2
   | _, _ => False
   end.
 
-Definition E' (P : nat -> AS.wval -> clval -> Prop) (W : web_map) (ex : bool) (i : nat) (ρ1 : AS.env) (ρ2 : cenv) (e : AS.exp) : Prop :=
+Definition E' (P : nat -> wval -> clval -> Prop) (W : web_map) (ex : bool) (i : nat) (ρ1 : env) (ρ2 : cenv) (e : exp) : Prop :=
   forall j1 r1,
     j1 <= i ->
-    AS.bstep_fuel ρ1 e j1 r1 ->
+    bstep_fuel ρ1 e j1 r1 ->
     exists j2 r2,
       cbstep_fuel W ex ρ2 e j2 r2 /\
         R' P (i - j1) r1 r2.
@@ -1648,22 +1646,23 @@ Definition E' (P : nat -> AS.wval -> clval -> Prop) (W : web_map) (ex : bool) (i
 (* W is sound for a particular program trace of e *)
 Definition web_map_sound W Γ ex ρ1 ρ2 e :=
   forall i r1,
-    AS.bstep_fuel ρ1 e i r1 ->
+    bstep_fuel ρ1 e i r1 ->
     refine_env Γ ρ1 ρ2 ->
     exists r2,
       cbstep_fuel W ex ρ2 e i r2 /\
         refine_res r1 r2.
 
-Fixpoint V (i : nat) (wv : AS.wval) (cv : clval) {struct i} : Prop :=
+Fixpoint V (i : nat) (wv : wval) (cv : clval) {struct i} : Prop :=
+  wf_val wv /\
   wf_cval cv /\
     refine_val wv cv /\
     match wv, cv with
-    | AS.TAG _ l1 v1, CTAG _ l2 W v2 =>
+    | TAG _ l1 v1, CTAG _ l2 W v2 =>
         l1 = l2 /\
           exists w2, W ! l2 = Some w2 /\
                        (w2 \in Exposed -> to_exposed cv) /\
                        match v1, v2 with
-                       | AS.Vconstr c1 vs1, CVconstr c2 vs2 =>
+                       | Vconstr c1 vs1, CVconstr c2 vs2 =>
                            c1 = c2 /\
                              length vs1 = length vs2 /\
                              match i with
@@ -1671,7 +1670,7 @@ Fixpoint V (i : nat) (wv : AS.wval) (cv : clval) {struct i} : Prop :=
                              | S i0 => Forall2 (V i0) vs1 vs2
                              end
 
-                       | AS.Vfun f1 ρ1 xs1 e1, CVfun f2 ρ2 xs2 e2 =>
+                       | Vfun f1 ρ1 xs1 e1, CVfun f2 ρ2 xs2 e2 =>
                            f1 = f2 /\
                              xs1 = xs2 /\
                              e1 = e2 /\
@@ -1682,9 +1681,9 @@ Fixpoint V (i : nat) (wv : AS.wval) (cv : clval) {struct i} : Prop :=
                                    j <= i0 ->
                                    (w2 \in Exposed -> Forall to_exposed vs2) ->
                                    Forall2 (V (i0 - (i0 - j))) vs1 vs2 ->
-                                   set_lists xs1 vs1 (M.set f1 (AS.Tag l1 (AS.Vfun f1 ρ1 xs1 e1)) ρ1) = Some ρ3 ->
+                                   set_lists xs1 vs1 (M.set f1 (Tag l1 (Vfun f1 ρ1 xs1 e1)) ρ1) = Some ρ3 ->
                                    set_lists xs2 vs2 (M.set f2 (CTag l2 W (CVfun f2 ρ2 xs2 e2)) ρ2) = Some ρ4 ->
-                                   web_map_sound W (AS.occurs_free e1) (exposedb w2) ρ3 ρ4 e1 ->
+                                   web_map_sound W (occurs_free e1) (exposedb w2) ρ3 ρ4 e1 ->
                                    E' V W (exposedb w2) (i0 - (i0 - j)) ρ3 ρ4 e1
                              end
 
@@ -1697,6 +1696,31 @@ Definition R := (R' V).
 Definition E := (E' V).
 
 (* Lemmas about [wf_cval], [wf_cres], and [wf_cenv] *)
+Lemma V_wf_val_l {i v1 v2}:
+  V i v1 v2 ->
+  wf_val v1.
+Proof. intros; destruct i; simpl in *; fcrush. Qed.
+
+Lemma V_wf_val_Forall_l {i vs1 vs2} :
+  Forall2 (V i) vs1 vs2 ->
+  Forall wf_val vs1.
+Proof. intros H. induction H; eauto using V_wf_val_l. Qed.
+
+Lemma V_wf_res_l {i v1 v2}:
+  V i v1 v2 ->
+  wf_res (Res v1).
+Proof. intros; eauto using V_wf_val_l; eauto. Qed.
+
+Lemma R_wf_res_l {i r1 r2} :
+  R i r1 r2 ->
+  wf_res r1.
+Proof.
+  unfold R.
+  intros.
+  destruct r1; destruct r2; try contradiction;
+    eauto using V_wf_val_l.
+Qed.
+
 Lemma V_wf_cval_r {i v1 v2}:
   V i v1 v2 ->
   wf_cval v2.
@@ -1747,63 +1771,69 @@ Qed.
 
 (* Inversion Lemmas *)
 Lemma R_res_inv_l i v1 r2 :
-  R i (AS.Res v1) r2 ->
+  R i (Res v1) r2 ->
   exists v2, r2 = CRes v2 /\ V i v1 v2.
 Proof. intros. fcrush. Qed.
 
 Lemma R_res_inv_l_V v1 r2 :
-  (forall k, R k (AS.Res v1) r2) ->
+  (forall k, R k (Res v1) r2) ->
   exists v2, r2 = CRes v2 /\ (forall k, V k v1 v2).
 Proof. intros. hauto. Qed.
 
 (* Environment Relation *)
-(* REVISIT: we don't need Γ2 *)
-Definition G i Γ1 ρ1 Γ2 ρ2 :=
+Definition G i Γ1 ρ1 ρ2 :=
+  wf_env ρ1 /\
   wf_cenv ρ2 /\
     refine_env Γ1 ρ1 ρ2 /\
     forall x,
       (x \in Γ1) ->
-      forall v1,
-        M.get x ρ1 = Some v1 ->
-        ((x \in Γ2) ->
-         exists v2,
-           M.get x ρ2 = Some v2 /\
-             V i v1 v2).
+      exists v1 v2,
+        M.get x ρ1 = Some v1 /\
+          M.get x ρ2 = Some v2 /\
+          V i v1 v2.
 
 (* Environment Lemmas *)
-Lemma G_subset Γ1 Γ2 {i ρ1 Γ3 ρ2 Γ4}:
-  G i Γ1 ρ1 Γ2 ρ2 ->
-  Γ3 \subset Γ1 ->
-  Γ4 \subset Γ2 ->
-  G i Γ3 ρ1 Γ4 ρ2.
+Lemma G_subset Γ1 Γ2 {i ρ1 ρ2}:
+  G i Γ1 ρ1 ρ2 ->
+  Γ2 \subset Γ1 ->
+  G i Γ2 ρ1 ρ2.
 Proof. unfold G. fcrush. Qed.
 
-Lemma G_wf_cenv_r {i Γ1 ρ1 Γ2 ρ2}:
-  G i Γ1 ρ1 Γ2 ρ2 ->
+Lemma G_wf_env_l {i Γ1 ρ1 ρ2}:
+  G i Γ1 ρ1 ρ2 ->
+  wf_env ρ1.
+Proof. unfold G. fcrush. Qed.
+
+Lemma G_wf_cenv_r {i Γ1 ρ1 ρ2}:
+  G i Γ1 ρ1 ρ2 ->
   wf_cenv ρ2.
 Proof. unfold G. fcrush. Qed.
 
-Lemma G_refine_env {i Γ1 ρ1 Γ2 ρ2}:
-  G i Γ1 ρ1 Γ2 ρ2 ->
+Lemma G_refine_env {i Γ1 ρ1 ρ2}:
+  G i Γ1 ρ1 ρ2 ->
   refine_env Γ1 ρ1 ρ2.
 Proof. unfold G. fcrush. Qed.
 
-Lemma G_get {Γ1 Γ2 i ρ1 ρ2}:
-  G i Γ1 ρ1 Γ2 ρ2 ->
+Lemma G_get {Γ1 i ρ1 ρ2}:
+  G i Γ1 ρ1 ρ2 ->
   forall x v1,
     (x \in Γ1) ->
-    (x \in Γ2) ->
     M.get x ρ1 = Some v1 ->
     exists v2,
       M.get x ρ2 = Some v2 /\
         V i v1 v2.
-Proof. unfold G. fcrush. Qed.
+Proof.
+  unfold G.
+  intros.
+  destruct H as [Hwf [Href HG]].
+  edestruct HG as [v1' [v2 [Heqv1 [Heqv2 HV]]]]; eauto; invc.
+  fcrush.
+Qed.
 
-Lemma G_get_list {i Γ1 ρ1 Γ2 ρ2} :
-  G i Γ1 ρ1 Γ2 ρ2 ->
+Lemma G_get_list {i Γ1 ρ1 ρ2} :
+  G i Γ1 ρ1 ρ2 ->
   forall xs vs1,
     (FromList xs) \subset Γ1 ->
-    (FromList xs) \subset Γ2 ->
     get_list xs ρ1 = Some vs1 ->
     exists vs2,
       get_list xs ρ2 = Some vs2 /\
@@ -1811,33 +1841,21 @@ Lemma G_get_list {i Γ1 ρ1 Γ2 ρ2} :
 Proof.
   intros HG xs.
   induction xs; simpl; intros.
-  - inv H1; eauto.
+  - fcrush.
   - destruct (ρ1 ! a) eqn:Heq1; try discriminate.
     destruct (get_list xs ρ1) eqn:Heq3; try discriminate.
-    inv H1.
+    inv H0.
     unfold Ensembles.Included, Ensembles.In in *.
     edestruct (G_get HG) as [v2 [Heqv2 HV]]; eauto.
-    eapply (H a).
-    apply in_eq.
-    apply H0.
-    apply in_eq.
-    edestruct IHxs as [vs2 [Heqvs2 Vvs]]; eauto.
-    + intros.
-      apply H.
-      apply in_cons; auto.
-    + intros.
-      apply H0.
-      apply in_cons; auto.
-    + rewrite Heqvs2.
-      exists (v2 :: vs2); split; auto.
-      rewrite Heqv2; auto.
+    eapply (H a); fcrush.
+    edestruct IHxs as [vs2 [Heqvs2 Vvs]]; eauto; fcrush.
 Qed.
 
-Lemma G_set {i Γ1 ρ1 Γ2 ρ2}:
-  G i Γ1 ρ1 Γ2 ρ2 ->
+Lemma G_set {i Γ1 ρ1 ρ2}:
+  G i Γ1 ρ1 ρ2 ->
   forall {x v1 v2},
     V i v1 v2 ->
-    G i (x |: Γ1) (M.set x v1 ρ1) (x |: Γ2) (M.set x v2 ρ2).
+    G i (x |: Γ1) (M.set x v1 ρ1) (M.set x v2 ρ2).
 Proof.
   unfold G.
   intro HG.
@@ -1846,28 +1864,33 @@ Proof.
 
   destruct HG as [Hwf [Href HG]].
   split.
+  eapply wf_env_set; eauto.
+  eapply V_wf_val_l; eauto.
+
+  split.
   eapply wf_cenv_set; eauto.
   eapply V_wf_cval_r; eauto.
 
   split.
   eapply refine_env_set; eauto.
+  eapply G_refine_env; eauto.
   eapply V_refine_val; eauto.
 
   intros.
   destruct (M.elt_eq x0 x); subst.
   - repeat rewrite M.gss in *.
     fcrush.
-  - rewrite M.gso in *; auto.
-    eapply G_get; eauto; fcrush.
+  - repeat (rewrite M.gso in *; auto).
+    fcrush.
 Qed.
 
-Lemma G_set_lists {i Γ1 ρ1 Γ2 ρ2}:
-  G i Γ1 ρ1 Γ2 ρ2 ->
+Lemma G_set_lists {i Γ1 ρ1 ρ2}:
+  G i Γ1 ρ1 ρ2 ->
   forall {xs vs1 vs2 ρ3 ρ4},
     Forall2 (V i) vs1 vs2 ->
     set_lists xs vs1 ρ1 = Some ρ3 ->
     set_lists xs vs2 ρ2 = Some ρ4 ->
-    G i (FromList xs :|: Γ1) ρ3 (FromList xs :|: Γ2) ρ4.
+    G i (FromList xs :|: Γ1) ρ3 ρ4.
 Proof.
   intros HG xs.
   induction xs; simpl; intros.
@@ -1882,7 +1905,7 @@ Proof.
     destruct (set_lists xs vs1 ρ1) eqn:Heq1; try discriminate.
     destruct (set_lists xs vs2 ρ2) eqn:Heq2; try discriminate.
     inv H; inv H0; inv H1.
-    eapply G_subset with (Γ1 := (a |: (FromList xs :|: Γ1))) (Γ2 := (a |: (FromList xs :|: Γ2))); eauto;
+    eapply G_subset with (Γ1 := (a |: (FromList xs :|: Γ1))); eauto;
       try (normalize_sets;
            rewrite Union_assoc;
            apply Included_refl).
@@ -1891,7 +1914,7 @@ Qed.
 
 (* Monotonicity Lemmas *)
 Lemma V_mono_Forall_aux :
-  forall i j (V : nat -> AS.wval -> clval -> Prop) vs1 vs2,
+  forall i j (V : nat -> wval -> clval -> Prop) vs1 vs2,
     (forall k : nat,
         k < S i ->
         forall (j : nat) v1 v2, V k v1 v2 -> j <= k -> V j v1 v2) ->
@@ -1918,7 +1941,7 @@ Proof.
   destruct i; simpl in H0;
     destruct j; simpl; intros;
     rename w into W;
-    destruct H0 as [Hwf [Href [Heql [w [Hw [Hex HV]]]]]]; subst.
+    destruct H0 as [Hwf1 [Hwf2 [Href [Heql [w [Hw [Hex HV]]]]]]]; subst.
   - destruct v; destruct c; fcrush.
   - fcrush.
   - repeat (split; auto).
@@ -1980,32 +2003,36 @@ Proof.
   apply R_mono with (i - j1); try lia; auto.
 Qed.
 
-Lemma G_mono {Γ1 Γ2 ρ1 ρ2} i j:
-  G i Γ1 ρ1 Γ2 ρ2 ->
+Lemma G_mono {Γ1 ρ1 ρ2} i j:
+  G i Γ1 ρ1 ρ2 ->
   j <= i ->
-  G j Γ1 ρ1 Γ2 ρ2.
+  G j Γ1 ρ1 ρ2.
 Proof.
   unfold G.
   intros.
-  destruct H as [Hwf [Href HG]].
+  destruct H as [Hwf1 [Hwf2 [Href HG]]].
   repeat (split; auto); intros.
-  edestruct HG as [v2 [Heqv2 HV]]; eauto.
+  edestruct HG as [v1 [v2 [Heqv1 [Heqv2 HV]]]]; eauto; invc.
   eexists; repeat (split; eauto).
   eauto using V_mono.
 Qed.
 
 (* Compatibility Lemmas *)
 Definition well_annotated W Γ e :=
+  occurs_free e \subset Γ /\
   forall ex i ρ1 ρ2,
     web_map_sound W Γ ex ρ1 ρ2 e ->
-    G i Γ ρ1 (AS.occurs_free e) ρ2 ->
+    G i Γ ρ1 ρ2 ->
     E W ex i ρ1 ρ2 e.
 
 Lemma ret_compat W Γ x :
   (x \in Γ) ->
-  well_annotated W Γ (AS.Eret x).
+  well_annotated W Γ (Eret x).
 Proof.
   unfold well_annotated, web_map_sound, E, E', R, R', Ensembles.Included, Ensembles.In.
+  split.
+  fcrush.
+
   intros; simpl.
   specialize (H0 _ _ H3).
   inv H3.
@@ -2034,16 +2061,15 @@ Proof.
   eapply refine_env_subset; eauto.
 Qed.
 
-Lemma Vfun_V W Γ1 f l w xs e  :
+Lemma Vfun_V W Γ f l w xs e  :
   W ! l = Some w ->
-  well_annotated W (FromList xs :|: (f |: Γ1)) e ->
-  forall {i Γ2 ρ1 ρ2},
+  well_annotated W (FromList xs :|: (f |: Γ)) e ->
+  forall {i ρ1 ρ2},
+    wf_val (Tag l (Vfun f ρ1 xs e)) ->
     wf_cval (CTag l W (CVfun f ρ2 xs e)) ->
-    refine_val (AS.Tag l (AS.Vfun f ρ1 xs e)) (CTag l W (CVfun f ρ2 xs e)) ->
-    G i Γ1 ρ1 Γ2 ρ2 ->
-    AS.occurs_free e \subset (FromList xs :|: (f |: Γ1)) ->
-    AS.occurs_free e \subset (FromList xs :|: (f |: Γ2)) ->
-    V i (AS.Tag l (AS.Vfun f ρ1 xs e)) (CTag l W (CVfun f ρ2 xs e)).
+    refine_val (Tag l (Vfun f ρ1 xs e)) (CTag l W (CVfun f ρ2 xs e)) ->
+    G i Γ ρ1 ρ2 ->
+    V i (Tag l (Vfun f ρ1 xs e)) (CTag l W (CVfun f ρ2 xs e)).
 Proof.
   unfold well_annotated.
   intros HW He i.
@@ -2051,24 +2077,25 @@ Proof.
     repeat (split; auto);
     intros; (repeat split; auto);
     eexists; repeat (split; eauto); intros.
+  destruct He as [HS He].
   apply (He _ (i - (i - j)) ρ3 ρ4); auto.
 
   eapply web_map_sound_subset; eauto.
 
-  eapply G_subset with (Γ2 := (FromList xs :|: (f |: Γ2))); eauto.
+  eapply G_subset; eauto.
   eapply G_set_lists; eauto.
   eapply G_set; eauto.
   + apply G_mono with (S i); eauto; lia.
   + apply V_mono with i; try lia.
-    eapply IHi with (Γ2 := Γ2); eauto.
+    eapply IHi; eauto.
     apply G_mono with (S i); eauto; lia.
-  + apply Included_refl.
+  + fcrush.
 Qed.
 
 Lemma web_map_sound_fun_inv_k W Γ ex ρ1 ρ2 f l xs e k:
-  web_map_sound W Γ ex ρ1 ρ2 (AS.Efun f l xs e k) ->
+  web_map_sound W Γ ex ρ1 ρ2 (Efun f l xs e k) ->
   refine_env Γ ρ1 ρ2 ->
-  web_map_sound W (f |: Γ) ex (M.set f (AS.Tag l (AS.Vfun f ρ1 xs e)) ρ1) (M.set f (CTag l W (CVfun f ρ2 xs e)) ρ2) k.
+  web_map_sound W (f |: Γ) ex (M.set f (Tag l (Vfun f ρ1 xs e)) ρ1) (M.set f (CTag l W (CVfun f ρ2 xs e)) ρ2) k.
 Proof.
   unfold web_map_sound.
   intros.
@@ -2077,15 +2104,20 @@ Proof.
   fcrush.
 Qed.
 
-(* TODO: make refine_env and G bidirectional *)
 Lemma fun_compat W Γ e k f l w xs :
   W ! l = Some w ->
   well_annotated W (FromList xs :|: (f |: Γ)) e ->
   well_annotated W (f |: Γ) k ->
-  well_annotated W Γ (AS.Efun f l xs e k).
+  well_annotated W Γ (Efun f l xs e k).
 Proof.
   unfold well_annotated, E, E'.
-  intros HWl He Hk.
+  intros HWl [HSe He] [HSk Hk].
+  split.
+  {
+    unfold Ensembles.Included, Ensembles.In in *.
+    intros.
+    inv H; fcrush.
+  }
   intros.
   pose proof H2 as Hbstep.
 
@@ -2093,27 +2125,22 @@ Proof.
   - exists 0, COOT; split; simpl; eauto.
   - destruct r1.
     fcrush.
+    assert (Hwfρ1 : wf_env ρ1) by eauto using G_wf_env_l.
+    assert (Hwfρ2 : wf_cenv ρ2) by eauto using G_wf_cenv_r.
     assert (Hrefρ : refine_env Γ ρ1 ρ2) by eauto using G_refine_env.
-    edestruct (H (S c) (AS.Res w0)) as [cv [Hcbstep Href]]; eauto.
+    edestruct (H (S c) (Res w0)) as [cv [Hcbstep Href]]; eauto.
 
     inv Hcbstep; inv H3.
     inv H4; invc.
-    edestruct (Hk ex (i - 1) (M.set f (AS.Tag l (AS.Vfun f ρ1 xs e)) ρ1) (M.set f (CTag l W (CVfun f ρ2 xs e)) ρ2)) with (j1 := c) (r1 := (AS.Res w0)) as [j2 [r2 [Hk2 Rr]]]; eauto; try lia.
+    edestruct (Hk ex (i - 1) (M.set f (Tag l (Vfun f ρ1 xs e)) ρ1) (M.set f (CTag l W (CVfun f ρ2 xs e)) ρ2)) with (j1 := c) (r1 := (Res w0)) as [j2 [r2 [Hk2 Rr]]]; eauto; try lia.
     + eauto using web_map_sound_fun_inv_k.
-    + eapply G_subset with (Γ2 := (f |: AS.occurs_free (AS.Efun f l xs e k))).
+    + eapply G_subset.
       eapply G_set; eauto.
       eapply G_mono with i; eauto; lia.
       * eapply Vfun_V; eauto.
-        -- eauto using G_wf_cenv_r.
         -- econstructor; eauto.
-           econstructor; eauto.
-           eapply Included_refl.
-           eapply AS.free_fun_e_inv; eauto.
-           admit.
         -- apply G_mono with i; eauto; lia.
-        -- apply AS.free_fun_e_subset.
       * apply Included_refl.
-      * apply AS.free_fun_k_subset.
     + exists (S j2), r2; split; auto.
       * econstructor; simpl; eauto.
         destruct ex; simpl in *; auto.
@@ -2121,14 +2148,11 @@ Proof.
       * eapply R_mono; eauto; lia.
 Qed.
 
-
-
-
 Lemma app_compat W Γ xs f l w :
   (W ! l = Some w) ->
   (f \in Γ) ->
   (FromList xs \subset Γ) ->
-  well_annotated W Γ (AS.Eapp f l xs).
+  well_annotated W Γ (Eapp f l xs).
 Proof.
   unfold well_annotated, E, E'.
   intros HW Hf Hxs.
@@ -2140,7 +2164,7 @@ Proof.
   - destruct r1.
     fcrush.
     assert (Hrefρ : refine_env ρ1 ρ2) by eauto using G_refine_env.
-    edestruct (H (S c) (AS.Res w0)) as [cv [Hcbstep Href]]; eauto.
+    edestruct (H (S c) (Res w0)) as [cv [Hcbstep Href]]; eauto.
     inv Hcbstep; inv H3; inv Href.
     inv H4; invc.
     edestruct (G_get H0 f) as [fv2 [Heqfv2 HV]]; eauto.
@@ -2152,7 +2176,7 @@ Proof.
       destruct HV as [Hwf [Hrefv [Heql [w2 [HW' [Hex [Heqf [Heqxs [Heqe HV]]]]]]]]]; subst; invc.
 
     edestruct (G_get_list H0 xs vs) as [vs2 [Heqvs2 Vvs]]; eauto; invc.
-    eapply AS.free_app_xs_subset; eauto.
+    eapply free_app_xs_subset; eauto.
 
     destruct (set_lists_length3 (M.set f'0 (CTag l0 W' (CVfun f'0 ρ'0 xs'0 e0)) ρ'0) xs'0 vs2) as [ρ4 Heqρ4].
     unfold clval in *.
@@ -2180,7 +2204,7 @@ Proof.
 
     apply (E_mono _ i) in HE; try lia.
     unfold E, E' in HE.
-    destruct (HE c (AS.Res v)) as [j2 [r2 [He0 Rr]]]; try lia; auto.
+    destruct (HE c (Res v)) as [j2 [r2 [He0 Rr]]]; try lia; auto.
     exists (S j2), r2; split; eauto.
 
     edestruct (R_res_inv_l _ _ _ Rr) as [cv' [Heqcv' HV']]; eauto; subst.
@@ -2197,7 +2221,7 @@ Lemma letapp_compat W Γ k xs x f l w :
   (f \in Γ) ->
   (FromList xs \subset Γ) ->
   well_annotated W (x |: Γ) k ->
-  well_annotated W Γ (AS.Eletapp x f l xs k).
+  well_annotated W Γ (Eletapp x f l xs k).
 Proof.
   unfold well_annotated, web_map_sound, E, E'.
   intros HWl Hf Hxs Hk.
@@ -2209,7 +2233,7 @@ Proof.
   - exists 0, COOT; split; simpl; auto.
   - destruct r1.
     fcrush.
-    edestruct (H (S c) (AS.Res w0)) as [cv [Hcbstep Href]]; eauto.
+    edestruct (H (S c) (Res w0)) as [cv [Hcbstep Href]]; eauto.
     inv Href.
     inv H3; inv Hcbstep.
     inv H3; invc.
@@ -2221,7 +2245,7 @@ Proof.
       destruct HV as [Hv1 [Href [Hl' [w2 [HW' [Hex [Heqf [Heqxs [Heqe HV]]]]]]]]]; invc.
 
     edestruct (G_get_list H0 xs vs) as [vs2 [Heqvs2 Vvs]]; eauto; invc.
-    eapply AS.free_letapp_xs_subset; eauto.
+    eapply free_letapp_xs_subset; eauto.
 
     destruct (set_lists_length3 (M.set f'0 (CTag l0 W' (CVfun f'0 ρ'0 xs'0 e0)) ρ'0) xs'0 vs2) as [ρ4 Heqρ4].
     {
@@ -2234,7 +2258,7 @@ Proof.
     {
       eapply bstep_fuel_cbstep_fuel_refine; eauto.
       assert (HVs : Forall2 refine_val vs vs2) by eauto using V_refine_val_Forall.
-      assert (Hrefenv : refine_env (M.set f'0 (AS.Tag l0 (AS.Vfun f'0 ρ' xs'0 e0)) ρ') (M.set f'0 (CTag l0 W' (CVfun f'0 ρ'0 xs'0 e0)) ρ'0)).
+      assert (Hrefenv : refine_env (M.set f'0 (Tag l0 (Vfun f'0 ρ' xs'0 e0)) ρ') (M.set f'0 (CTag l0 W' (CVfun f'0 ρ'0 xs'0 e0)) ρ'0)).
       {
         eapply refine_env_set; eauto.
         inv Href.
@@ -2255,7 +2279,7 @@ Proof.
 
       unfold web_map_sound; intros.
       destruct r1.
-      - edestruct (H (S i0) AS.OOT) as [r2 [Hcbstep_e Hrefr]]; eauto.
+      - edestruct (H (S i0) OOT) as [r2 [Hcbstep_e Hrefr]]; eauto.
         inv Hcbstep_e.
         inv Hrefr.
         inv H8.
@@ -2266,22 +2290,22 @@ Proof.
           eapply bstep_fuel_cbstep_fuel_refine; eauto.
         }
         inv Hc.
-        eapply AS.bstep_fuel_lt_Res_not_OOT with (c0 := (c0 + c'0)) in H14; eauto; try lia.
+        eapply bstep_fuel_lt_Res_not_OOT with (c0 := (c0 + c'0)) in H14; eauto; try lia.
         contradiction.
 
         unfold clval in *; invc; eauto.
       - assert (Hcv : v = w /\ c = i0).
         {
-          eapply AS.bstep_fuel_deterministic; eauto.
+          eapply bstep_fuel_deterministic; eauto.
         }
         inv Hcv.
 
-        edestruct (H (S (i0 + c')) (AS.Res w0)) as [r2 [Hcbstep_e Hrefr]]; eauto.
+        edestruct (H (S (i0 + c')) (Res w0)) as [r2 [Hcbstep_e Hrefr]]; eauto.
     }
 
     apply (E_mono _ i) in HE; try lia.
     unfold E in HE.
-    destruct (HE c (AS.Res v)) as [j1 [ra [Hap Rra]]]; try lia; auto.
+    destruct (HE c (Res v)) as [j1 [ra [Hap Rra]]]; try lia; auto.
 
     simpl in Rra.
     destruct ra; try contradiction.
@@ -2293,7 +2317,7 @@ Proof.
     inv Heq.
 
     edestruct (Hk ex (i - c) (M.set x v ρ1) (M.set x v0 ρ2))
-      with (j1 := c') (r1 := (AS.Res w0)) as [j2 [r2 [Hk2 Rr]]]; eauto; try lia.
+      with (j1 := c') (r1 := (Res w0)) as [j2 [r2 [Hk2 Rr]]]; eauto; try lia.
     + intros.
 
       edestruct (H (S (c + i0)) r1) as [r2 [Hcbstep2 Href2]]; eauto.
@@ -2309,11 +2333,11 @@ Proof.
       * inv Href2.
         eapply cbstep_fuel_lt_Res_not_OOT with (c0 := (c + i0)) in Hap; eauto; try lia.
         contradiction.
-    + eapply G_subset with (Γ2 := (x |: (AS.occurs_free (AS.Eletapp x f l xs k)))).
+    + eapply G_subset with (Γ2 := (x |: (occurs_free (Eletapp x f l xs k)))).
       ++ eapply G_set; eauto.
          eapply G_mono with (S i); eauto; lia.
       ++ apply Included_refl.
-      ++ apply AS.free_letapp_k_subset.
+      ++ apply free_letapp_k_subset.
     + exists (S (c + j2)), r2; split.
       ++ constructor; auto.
          ** econstructor; eauto.
@@ -2327,7 +2351,7 @@ Qed.
 Lemma case_nil_compat W Γ x l w :
   W ! l = Some w ->
   (x \in Γ) ->
-  well_annotated W Γ (AS.Ecase x l []).
+  well_annotated W Γ (Ecase x l []).
 Proof.
   unfold well_annotated, E, E'.
   intros HWl Hx.
@@ -2355,7 +2379,7 @@ Admitted.
 
 (* Top-level Compilation Unit & Linking *)
 Inductive cexp : Type :=
-| CEexp : web_map -> AS.exp -> cexp
+| CEexp : web_map -> exp -> cexp
 | CElink : var -> cexp -> cexp -> cexp.
 
 Hint Constructors cexp : core.
@@ -2366,7 +2390,7 @@ Definition link x e1 e2 : cexp := CElink x e1 e2.
 Inductive occurs_free_top : cexp -> vars :=
 | Free_cexp :
   forall W e x,
-    AS.occurs_free e x ->
+    occurs_free e x ->
     occurs_free_top (CEexp W e) x
 
 | Free_clink1 :
@@ -2383,7 +2407,7 @@ Inductive occurs_free_top : cexp -> vars :=
 Hint Constructors occurs_free_top : core.
 
 Lemma occurs_free_top_cexp W e :
-  (occurs_free_top (CEexp W e)) <--> (AS.occurs_free e).
+  (occurs_free_top (CEexp W e)) <--> (occurs_free e).
 Proof. split; unfold Ensembles.Included, Ensembles.In; fcrush. Qed.
 
 (* Top-level Checking Semantics *)
@@ -2495,7 +2519,7 @@ Proof.
     intros Hρ2 HFV Hsub Hcb.
     inv Hcb.
     + (* Cbstep_exp_top *)
-      assert (HFV' : AS.occurs_free e0 \subset Γ).
+      assert (HFV' : occurs_free e0 \subset Γ).
       { unfold Ensembles.Included, Ensembles.In in *. intros z Hz.
         apply HFV. constructor; auto. }
       edestruct (cbstep_subenv Hρ2 HFV' Hsub H) as [r2 [Hr2 [Hsr Hwfr]]].
@@ -2560,23 +2584,23 @@ Qed.
 
 (* Cross-language Logical Relations *)
 
-Definition E_top' (P : nat -> AS.wval -> clval -> Prop) (i : nat) (ρ1 : AS.env) (e1 : AS.exp) (ρ2 : cenv) (e2 : cexp) : Prop :=
+Definition E_top' (P : nat -> wval -> clval -> Prop) (i : nat) (ρ1 : env) (e1 : exp) (ρ2 : cenv) (e2 : cexp) : Prop :=
   forall j1 r1,
     j1 <= i ->
-    AS.bstep_fuel ρ1 e1 j1 r1 ->
+    bstep_fuel ρ1 e1 j1 r1 ->
     exists j2 r2,
       cbstep_top_fuel ρ2 e2 j2 r2 /\
       R' P (i - j1) r1 r2.
 
-Fixpoint V_top (i : nat) (wv : AS.wval) (cv : clval) {struct i} : Prop :=
+Fixpoint V_top (i : nat) (wv : wval) (cv : clval) {struct i} : Prop :=
   wf_cval cv /\
     refine_val wv cv /\
     to_exposed cv /\
     match wv, cv with
-    | AS.TAG _ l1 v1, CTAG _ l2 W v2 =>
+    | TAG _ l1 v1, CTAG _ l2 W v2 =>
         l1 = l2 /\
           match v1, v2 with
-          | AS.Vconstr c1 vs1, CVconstr c2 vs2 =>
+          | Vconstr c1 vs1, CVconstr c2 vs2 =>
               c1 = c2 /\
                 length vs1 = length vs2 /\
                 match i with
@@ -2584,7 +2608,7 @@ Fixpoint V_top (i : nat) (wv : AS.wval) (cv : clval) {struct i} : Prop :=
                 | S i0 => Forall2 (V_top i0) vs1 vs2
                 end
 
-          | AS.Vfun f1 ρ1 xs1 e1, CVfun f2 ρ2 xs2 e2 =>
+          | Vfun f1 ρ1 xs1 e1, CVfun f2 ρ2 xs2 e2 =>
               f1 = f2 /\
                 xs1 = xs2 /\
                 e1 = e2 /\
@@ -2595,7 +2619,7 @@ Fixpoint V_top (i : nat) (wv : AS.wval) (cv : clval) {struct i} : Prop :=
                       j <= i0 ->
                       Forall to_exposed vs2 ->
                       Forall2 (V_top (i0 - (i0 - j))) vs1 vs2 ->
-                      set_lists xs1 vs1 (M.set f1 (AS.Tag l1 (AS.Vfun f1 ρ1 xs1 e1)) ρ1) = Some ρ3 ->
+                      set_lists xs1 vs1 (M.set f1 (Tag l1 (Vfun f1 ρ1 xs1 e1)) ρ1) = Some ρ3 ->
                       set_lists xs2 vs2 (M.set f2 (CTag l2 W (CVfun f2 ρ2 xs2 e2)) ρ2) = Some ρ4 ->
                       web_map_sound W true ρ3 ρ4 e1 ->
                       E_top' V_top (i0 - (i0 - j)) ρ3 e1 ρ4 (CEexp W e1)
@@ -2808,7 +2832,7 @@ Qed.
 
 (* Top-level Inversion Lemmas *)
 Lemma R_top_res_inv_l i v1 r2 :
-  R_top i (AS.Res v1) r2 ->
+  R_top i (Res v1) r2 ->
   exists v2, r2 = CRes v2 /\ V_top i v1 v2.
 Proof.
   intros.
@@ -2817,7 +2841,7 @@ Proof.
 Qed.
 
 Lemma R_top_res_inv_l_V v1 r2 :
-  (forall k, R_top k (AS.Res v1) r2) ->
+  (forall k, R_top k (Res v1) r2) ->
   exists v2, r2 = CRes v2 /\ (forall k, V_top k v1 v2).
 Proof. intros. hauto. Qed.
 
@@ -3063,7 +3087,7 @@ Qed.
 (* W is sound for *every* program trace of an open program e *)
 Definition web_map_sound_top e e' :=
   forall i ρ1 ρ2 r1,
-    AS.bstep_fuel ρ1 e i r1 ->
+    bstep_fuel ρ1 e i r1 ->
     refine_env ρ1 ρ2 ->
     wf_cenv ρ2 ->
     exists r2,
@@ -3097,19 +3121,19 @@ Proof.
 Qed.
 
 Definition trans_correct_top e e' :=
-  (occurs_free_top e') \subset (AS.occurs_free e) /\
+  (occurs_free_top e') \subset (occurs_free e) /\
   web_map_sound_top e e' /\
   forall i ρ1 ρ2,
-    G_top i (AS.occurs_free e) ρ1 (occurs_free_top e') ρ2 ->
+    G_top i (occurs_free e) ρ1 (occurs_free_top e') ρ2 ->
     E_top i ρ1 e ρ2 e'.
 
 Lemma trans_correct_top_subset e1 e2 :
   trans_correct_top e1 e2 ->
-  occurs_free_top e2 \subset AS.occurs_free e1.
+  occurs_free_top e2 \subset occurs_free e1.
 Proof. unfold trans_correct_top. fcrush. Qed.
 
 Lemma cexp_compat_top W e :
-  web_map_spec W (AS.occurs_free e) e ->
+  web_map_spec W (occurs_free e) e ->
   web_map_sound_top e (CEexp W e) ->
   trans_correct_top e (CEexp W e).
 Proof.
@@ -3141,37 +3165,37 @@ Qed.
 Lemma trans_correct_top_trans_correct W e :
   web_map_sound_top e (CEexp W e) ->
   trans_correct_top e (CEexp W e) ->
-  well_annotated W (AS.occurs_free e) e.
+  well_annotated W (occurs_free e) e.
 Proof.
 Abort.
 
 Lemma web_map_sound_top_preserves_linking f x e1 e1' e2 e2' :
   f <> x ->
-  ~ (f \in AS.occurs_free e1) ->
-  ~ (f \in AS.occurs_free e2) ->
+  ~ (f \in occurs_free e1) ->
+  ~ (f \in occurs_free e2) ->
   ~ (f \in occurs_free_top e1') ->
   ~ (f \in occurs_free_top e2') ->
   web_map_sound_top e1 e1' ->
   web_map_sound_top e2 e2' ->
-  web_map_sound_top (AS.link f x e1 e2) (link x e1' e2').
+  web_map_sound_top (link f x e1 e2) (link x e1' e2').
 Proof.
   intros Hfx Hf1 Hf2 Hf1' Hf2' H1 H2.
-  unfold AS.link, link.
+  unfold link, link.
   unfold web_map_sound_top in *.
   intros i ρ1 ρ2 r1 Hbstep Href Hwfρ2.
   inv Hbstep.
   { exists COOT; split; eauto. }
   match goal with
-  | [ H : AS.bstep _ _ _ _ |- _ ] => inv H
+  | [ H : bstep _ _ _ _ |- _ ] => inv H
   end.
   match goal with
-  | [ H : AS.bstep_fuel _ (AS.Eletapp _ _ _ _ _) _ _ |- _ ] => inv H
+  | [ H : bstep_fuel _ (Eletapp _ _ _ _ _) _ _ |- _ ] => inv H
   end.
   { (* trivially-OOT Eletapp: source fuel = 1 *)
     exists COOT; split; [|constructor].
     apply CbstepTF_Step; [apply Cbstep_link_top_trivial | constructor]. }
   match goal with
-  | [ H : AS.bstep _ (AS.Eletapp _ _ _ _ _) _ _ |- _ ] => inv H
+  | [ H : bstep _ (Eletapp _ _ _ _ _) _ _ |- _ ] => inv H
   end;
     match goal with
     | [ H : M.get _ (M.set _ _ _) = Some _ |- _ ] =>
@@ -3185,17 +3209,17 @@ Proof.
     end.
   - (* BStep_letapp_Res *)
     match goal with
-    | [ Hb : AS.bstep_fuel _ _ _ (AS.Res _) |- _ ] => rename Hb into Hbody
+    | [ Hb : bstep_fuel _ _ _ (Res _) |- _ ] => rename Hb into Hbody
     end.
     match goal with
-    | [ Hk : AS.bstep_fuel _ e2 _ _ |- _ ] => rename Hk into Hcont
+    | [ Hk : bstep_fuel _ e2 _ _ |- _ ] => rename Hk into Hcont
     end.
     rename f' into f.
     rename ρ' into ρ1.
     rename e into e1.
-    assert (Hwf1 : AS.wf_env ρ1) by admit.
+    assert (Hwf1 : wf_env ρ1) by admit.
 
-    edestruct (AS.bstep_fuel_drop_unused Hf1 Hwf1 Hbody) as [r1' [Hbstep_e1 Hsub']]; eauto.
+    edestruct (bstep_fuel_drop_unused Hf1 Hwf1 Hbody) as [r1' [Hbstep_e1 Hsub']]; eauto.
     inv Hsub'.
 
     edestruct H1 as [r2 [Hcbstep_e1' Href']]; eauto.
@@ -3203,26 +3227,26 @@ Proof.
 
     rewrite (set_set x f) in Hcont; auto.
 
-    assert (Hwfv : AS.wf_res (AS.Res v)).
+    assert (Hwfv : wf_res (Res v)).
     {
-      eapply AS.bstep_fuel_wf_res; eauto.
+      eapply bstep_fuel_wf_res; eauto.
     }
 
-    assert (Hwf2 : AS.wf_env (M.set x v ρ1)).
+    assert (Hwf2 : wf_env (M.set x v ρ1)).
     {
-      eapply AS.wf_env_set; eauto.
+      eapply wf_env_set; eauto.
       inv Hwfv; auto.
     }
 
-    edestruct (AS.bstep_fuel_drop_unused Hf2 Hwf2 Hcont) as [r2' [Hbstep_e2 Hsub2']]; eauto.
+    edestruct (bstep_fuel_drop_unused Hf2 Hwf2 Hcont) as [r2' [Hbstep_e2 Hsub2']]; eauto.
 
-    assert (Hsub3 : AS.subenv (x |: AS.occurs_free e2) (M.set x v ρ1) (M.set x v2 ρ1)).
+    assert (Hsub3 : subenv (x |: occurs_free e2) (M.set x v ρ1) (M.set x v2 ρ1)).
     {
-      eapply AS.subenv_set; eauto.
-      eapply AS.subenv_refl; eauto.
+      eapply subenv_set; eauto.
+      eapply subenv_refl; eauto.
     }
 
-    edestruct @AS.bstep_fuel_subenv with (Γ := (x |: AS.occurs_free e2)) as [r2'' [Hbstep_e2' Hsub2'']]; eauto.
+    edestruct @bstep_fuel_subenv with (Γ := (x |: occurs_free e2)) as [r2'' [Hbstep_e2' Hsub2'']]; eauto.
     fcrush.
 
     edestruct (H2 c' (M.set x v2 ρ1) (M.set x v' ρ2)) as [r2''' [Hcbstep_e2' Href'']]; eauto.
@@ -3239,20 +3263,20 @@ Proof.
     econstructor; eauto.
     inv Hcbstep_e2'; auto.
 
-    assert (Hsubres : AS.subres r1 r2'') by eauto using AS.subres_trans.
+    assert (Hsubres : subres r1 r2'') by eauto using subres_trans.
     (* need a lemma for refine_res and subres *)
     admit.
 Admitted.
 
 Lemma preserves_linking f x e1 e1' e2 e2' :
   f <> x ->
-  ~ (f \in AS.occurs_free e1) ->
-  ~ (f \in AS.occurs_free e2) ->
+  ~ (f \in occurs_free e1) ->
+  ~ (f \in occurs_free e2) ->
   ~ (f \in occurs_free_top e1') ->
   ~ (f \in occurs_free_top e2') ->
   trans_correct_top e1 e1' ->
   trans_correct_top e2 e2' ->
-  trans_correct_top (AS.link f x e1 e2) (link x e1' e2').
+  trans_correct_top (link f x e1 e2) (link x e1' e2').
 Proof.
   intros Hfx Hf1 Hf2 Hf1' Hf2' Htr1 Htr2.
   destruct Htr1 as [HFV1 [Hsnd1 HE1]].
@@ -3260,28 +3284,28 @@ Proof.
   unfold trans_correct_top.
   repeat split.
 
-  - (* FV inclusion: occurs_free_top (link x e1' e2') ⊆ AS.occurs_free (AS.link f x e1 e2) *)
-    unfold AS.link, link.
+  - (* FV inclusion: occurs_free_top (link x e1' e2') ⊆ occurs_free (link f x e1 e2) *)
+    unfold link, link.
     unfold Ensembles.Included, Ensembles.In.
     intros z Hz.
     inv Hz.
     + (* Free_clink1: z ∈ FV(e1'); need z ∈ FV(Efun f l0 [] e1 _) via Free_fun2 *)
       assert (Hne : z <> f) by (intros ?; subst; apply Hf1'; auto).
-      apply AS.Free_fun2.
+      apply Free_fun2.
       * auto.
       * intros Hin; inv Hin.
       * apply HFV1; auto.
     + (* Free_clink2: z ≠ x ∧ z ∈ FV(e2'); need z ∈ FV(Efun ...) via Free_fun1 + Free_letapp1 *)
       assert (Hne : z <> f) by (intros ?; subst; apply Hf2'; auto).
-      apply AS.Free_fun1.
+      apply Free_fun1.
       * auto.
-      * apply AS.Free_letapp1; auto.
+      * apply Free_letapp1; auto.
         apply HFV2; auto.
 
   - eapply web_map_sound_top_preserves_linking; eauto.
 
   - intros i ρ1 ρ2 HG.
-    unfold AS.link, link, E_top, E_top' in *.
+    unfold link, link, E_top, E_top' in *.
     intros.
     inv H0.
     fcrush.
@@ -3294,9 +3318,9 @@ Proof.
     rename f' into f.
     rename ρ' into ρ1.
 
-    assert (Hwf1 : AS.wf_env ρ1) by admit.
+    assert (Hwf1 : wf_env ρ1) by admit.
 
-    edestruct (AS.bstep_fuel_drop_unused Hf1 Hwf1 H11) as [r1' [Hbstep_e1 Hsub']]; eauto.
+    edestruct (bstep_fuel_drop_unused Hf1 Hwf1 H11) as [r1' [Hbstep_e1 Hsub']]; eauto.
     inv Hsub'.
 
     edestruct (HE1 i ρ1 ρ2) with (j1 := c) as [j1 [r1' [Hcbstep_e1' HR1']]]; eauto; try lia.
@@ -3310,23 +3334,23 @@ Proof.
 
     rewrite (set_set x f) in H12; auto.
 
-    assert (Hwfv : AS.wf_res (AS.Res v)) by eauto using AS.bstep_fuel_wf_res; eauto.
+    assert (Hwfv : wf_res (Res v)) by eauto using bstep_fuel_wf_res; eauto.
 
-    assert (Hwf2 : AS.wf_env (M.set x v ρ1)).
+    assert (Hwf2 : wf_env (M.set x v ρ1)).
     {
-      eapply AS.wf_env_set; eauto.
+      eapply wf_env_set; eauto.
       inv Hwfv; auto.
     }
 
-    edestruct (AS.bstep_fuel_drop_unused Hf2 Hwf2 H12) as [r2' [Hbstep_e2 Hsub']]; eauto.
+    edestruct (bstep_fuel_drop_unused Hf2 Hwf2 H12) as [r2' [Hbstep_e2 Hsub']]; eauto.
 
-    assert (Hsub3 : AS.subenv (x |: AS.occurs_free e2) (M.set x v ρ1) (M.set x v2 ρ1)).
+    assert (Hsub3 : subenv (x |: occurs_free e2) (M.set x v ρ1) (M.set x v2 ρ1)).
     {
-      eapply AS.subenv_set; eauto.
-      eapply AS.subenv_refl; eauto.
+      eapply subenv_set; eauto.
+      eapply subenv_refl; eauto.
     }
 
-    edestruct @AS.bstep_fuel_subenv with (Γ := (x |: AS.occurs_free e2)) as [r2'' [Hbstep_e2' Hsub2'']]; eauto.
+    edestruct @bstep_fuel_subenv with (Γ := (x |: occurs_free e2)) as [r2'' [Hbstep_e2' Hsub2'']]; eauto.
     fcrush.
 
     edestruct (HE2 (i - c) (M.set x v2 ρ1) (M.set x v2' ρ2)) with (j1 := c') as [j2'' [r2''' [Hcbstep_e2' Href'']]]; eauto; try lia.
@@ -3348,7 +3372,7 @@ Proof.
     econstructor; eauto.
     eapply cbstep_top_fuel_exposed_inv; eauto.
 
-    assert (Hsubres : AS.subres r1 r2'') by eauto using AS.subres_trans.
+    assert (Hsubres : subres r1 r2'') by eauto using subres_trans.
 
     (* need a lemma for V_top and subval *)
     (* eapply R_top_mono; eauto. *)
@@ -3386,24 +3410,4 @@ Lemma V_top_subval :
 Proof.
   intro i.
   induction i using lt_wf_rec; intros v1 v2 v3 Hsub.
-  (* The proof follows V_V_top's structure: strong induction on i, then
-     destruct i (= 0 vs S i'), destructure values, recurse via IH for
-     subterms.
-
-     Key obstacles (not trivially closeable):
-
-     1. [refine_val] (a conjunct of V_top) does not compose with [subval]
-        in general. For Vfun, refine_val (Tag w (Vfun f ρ1 xs e)) v3 is
-        [refine_env ρ1 ρ_c]; under subval' (Vfun f ρ1 xs e) (Vfun f ρ2 xs e)
-        (via [subenv Γ ρ1 ρ2]) we cannot conclude [refine_env ρ2 ρ_c]
-        because Dom(ρ2) may extend beyond Γ where ρ_c offers no coverage.
-
-     2. The Vfun behavioral conjunct (E_top' relation under set_lists) needs
-        the AS-side bstep behavior to transfer between ρ_a- and ρ_b-based
-        envs. [bstep_subenv] supplies this but threading it requires
-        composing with V_top_subval at smaller indices.
-
-     A fully honest fix is to parameterize refine_val/refine_env by a domain
-     (analogous to csubenv's Γ) so refine_val ↔ subval composition holds in
-     both directions. Left admitted as a focused gap. *)
 Admitted.
